{
  "@context": {
    "airline": "http://williamrobertfunk.com/ontologies/airline#",
    "airport": "http://williamrobertfunk.com/ontologies/airport#",
    "blade": "http://modusoperandi.com/ont/blade#",
    "country": "http://williamrobertfunk.com/ontologies/country#",
    "dc": "http://purl.org/dc/elements/1.1/",
    "owl": "http://www.w3.org/2002/07/owl#",
    "rdf": "http://www.w3.org/1999/02/22-rdf-syntax-ns#",
    "rdfs": "http://www.w3.org/2000/01/rdf-schema#",
    "xsd": "http://www.w3.org/2001/XMLSchema#"
  },
  "@graph": [
    {
      "@id": "country:hasCountry",
      "@type": "owl:ObjectProperty",
      "rdfs:domain": {
        "@id": "airline:GovernmentOffice"
      },
      "rdfs:range": {
        "@id": "country:Country"
      }
    },
    {
      "@id": "airport:iataCode",
      "@type": [
        "owl:DatatypeProperty",
        "owl:FunctionalProperty"
      ],
      "rdfs:comment": "\n      The International Air Transportation Association code associated with an airport or airline.\n    ",
      "rdfs:domain": {
        "@id": "airline:Airline"
      },
      "rdfs:label": "IATA Code",
      "rdfs:range": {
        "@id": "xsd:string"
      }
    },
    {
      "@id": "airline:callsign",
      "@type": "owl:DatatypeProperty",
      "rdfs:comment": "\n      A message, code, or tune that is broadcast by radio to identify the broadcaster or transmitter.\n    ",
      "rdfs:domain": {
        "@id": "airline:Airline"
      },
      "rdfs:label": "Callsign",
      "rdfs:range": {
        "@id": "xsd:string"
      }
    },
    {
      "@id": "airline:Airline",
      "@type": "owl:Class",
      "blade:navClass": true,
      "rdfs:comment": "\n      An organization providing a regular public service of air transportation on one or more routes.\n    ",
      "rdfs:label": "Airline"
    },
    {
      "@id": "airport:icaoCode",
      "@type": [
        "owl:DatatypeProperty",
        "owl:FunctionalProperty"
      ],
      "rdfs:comment": "\n      The International Civil Aviation Organization code associated with an airport.\n    ",
      "rdfs:domain": {
        "@id": "airline:Airline"
      },
      "rdfs:label": "ICAO Code",
      "rdfs:range": {
        "@id": "xsd:string"
      }
    },
    {
      "@id": "airline:name",
      "@type": "owl:DatatypeProperty",
      "rdfs:comment": "\n      An alternate word or set of words by which an airline is known, referred to, or addressed.\n    ",
      "rdfs:domain": {
        "@id": "airline:Airline"
      },
      "rdfs:label": "Name",
      "rdfs:range": {
        "@id": "xsd:string"
      }
    },
    {
      "@id": "airline:status",
      "@type": [
        "owl:DatatypeProperty",
        "owl:FunctionalProperty"
      ],
      "rdfs:comment": "\n      The last known status of the airline (ie. operational or defunct).\n    ",
      "rdfs:domain": {
        "@id": "airline:Airline"
      },
      "rdfs:label": "Status",
      "rdfs:range": {
        "@id": "xsd:string"
      }
    },
    {
      "@id": "http://williamrobertfunk.com/ontologies/airline",
      "@type": "owl:Ontology",
      "dc:contributor": "William R.A.D. Funk",
      "dc:creator": "William R.A.D. Funk",
      "dc:rights": "Copyright 2019 William R.A.D. Funk. All rights reserved.",
      "owl:versionInfo": {
        "@type": "xsd:decimal",
        "@value": "1.0"
      },
      "rdfs:comment": "\n      Identifies application specific classes and annotations that are relevant\n      only to my associated applications.\n    ",
      "rdfs:label": "Funk Ontology"
    },
    {
      "@id": "airline:alias",
      "@type": "owl:DatatypeProperty",
      "rdfs:comment": "\n      A word or set of words by which an airline is known, referred to, or addressed.\n    ",
      "rdfs:domain": {
        "@id": "airline:Airline"
      },
      "rdfs:label": "Alias",
      "rdfs:range": {
        "@id": "xsd:string"
      }
    }
  ]
}